\section{Prob 4. b)}

The linear growth factor can be calculated indirectly from
\begin{equation}\label{eq:1}
    \dot D(t) = \frac{dD}{da} \dot a, 
\end{equation}
where $\dot a(z) = H(z)a(z)$. Plug in $\dot a(z)$ and rewrite the equation with the chain rule, \cref{eq:1} then becomes
\begin{equation}\label{eq:2}
    \dot D(z) = \frac{dD}{da} H(z) a(z) = \frac{dD}{da} \frac{H(z)}{1+z} = \frac{dD}{dz} \frac{dz}{da} \frac{H(z)}{1+z},
\end{equation}
where $a(z) = \frac{1}{1+z}$. Take the derivative of $a$ with respect of $z$, we have
\begin{equation}
    \frac{da}{dz} = - \frac{1}{(1+z)^2} \quad
    \Rightarrow \quad \frac{dz}{da} = - (1+z)^2
\end{equation}
Thus, we can simplify \cref{eq:2} to 
\begin{equation}\label{eq:4}
    \dot D(z) = - \frac{dD}{dz} (1+z) H(z).
\end{equation}
From part a) we get the linear growth factor and the Hubble parameter as a function, 
\begin{gather}
    D(z) = \frac{5 \Omega_m {H_0}^2 }{2} H(z) \int_{z}^{\infty} \frac{1+z'}{H^3(z')} dz' \\
    H(z) = (\Omega_m (1+z)^3 + \Omega_{\Lambda})^{1/2}.
\end{gather}
Their derivatives with respect to $z$ are then,
\begin{gather}
    \label{eq:7}
    \frac{dD}{dz} = \frac{5 \Omega_m {H_0}^2 }{2} [\frac{dH(z)}{dz} \int_{z}^{\infty} \frac{1+z'}{H^3(z')} dz' + H(z) \frac{d}{dz} \int_{z}^{\infty} \frac{1+z'}{H^3(z')} dz'] \\ 
    \label{eq:8}
    \frac{dH}{dz} = \frac{3 \Omega_m (1+z)^2}{2[\Omega_m (1+z)^3 + \Omega_\Lambda]^{1/2}}.
\end{gather}
Substitute \cref{eq:7} and \cref{eq:8} into \cref{eq:4} and simplify, we get 
\begin{equation}\label{eq:9}
\begin{split}
    \dot D(z) &= - \frac{5 \Omega_m {H_0}^2 }{2} [\frac{dH(z)}{dz} \int_{z}^{\infty} \frac{1+z'}{H^3(z')} dz' + H(z) \frac{d}{dz} \int_{z}^{\infty} \frac{1+z'}{H^3(z')} dz'] (1+z) H(z) \\
    &= - \frac{5 \Omega_m {H_0}^2 }{2}  (\frac{3 \Omega_m (1+z)^2}{2[\Omega_m (1+z)^3 + \Omega_\Lambda]^{1/2}} \int_{z}^{\infty} \frac{1+z'}{H^3(z')} dz' + \\
    &\qquad \qquad \qquad \frac{(1+z)^2}{[\Omega_m (1+z)^3 + \Omega_\Lambda]^{1/2}}) \cdot (1+z) [\Omega_m (1+z)^3 + \Omega_\Lambda]^{1/2} \\
    &= - \frac{5 \Omega_m {H_0}^2 }{2} (\frac{3 \Omega_m (1+z)^3}{2} \int_{z}^{\infty} \frac{1+z'}{H^3(z')} dz' + \frac{(1+z)^2}{[\Omega_m (1+z)^3 + \Omega_\Lambda]^{1/2}}).
\end{split}
\end{equation}
\cref{eq:9} is then what we need for the time derivative of the linear growth factor $D$ as a function of the redshift $z$. 